<?xml version="1.0"?>
<rdf:RDF xmlns="http://geographicknowledge.de/vocab/CoreConceptData.rdf#"
     xml:base="http://geographicknowledge.de/vocab/CoreConceptData.rdf"
     xmlns:owl="http://www.w3.org/2002/07/owl#"
     xmlns:rdf="http://www.w3.org/1999/02/22-rdf-syntax-ns#"
     xmlns:xml="http://www.w3.org/XML/1998/namespace"
     xmlns:xsd="http://www.w3.org/2001/XMLSchema#"
     xmlns:rdfs="http://www.w3.org/2000/01/rdf-schema#">
    <owl:Ontology rdf:about="http://geographicknowledge.de/vocab/CoreConceptData.rdf">
        <owl:imports rdf:resource="http://geographicknowledge.de/vocab/AnalysisData.rdf"/>
        <rdfs:comment xml:lang="en">This ontology pattern describes geodata types representing core concepts of spatial information (Kuhn 2012) we well as further semantic attribute distinctions relevant for geocomputation and geo-analysis.</rdfs:comment>
        <rdfs:seeAlso rdf:resource="http://spatial.ucsb.edu/core-concepts-of-spatial-information/"/>
    </owl:Ontology>
    


    <!-- 
    ///////////////////////////////////////////////////////////////////////////////////////
    //
    // Classes
    //
    ///////////////////////////////////////////////////////////////////////////////////////
     -->

    


    <!-- http://geographicknowledge.de/vocab/AnalysisData.rdf#Attribute -->

    <rdf:Description rdf:about="http://geographicknowledge.de/vocab/AnalysisData.rdf#Attribute">
        <owl:equivalentClass rdf:resource="http://geographicknowledge.de/vocab/CoreConceptData.rdf#Attribute"/>
    </rdf:Description>
    


    <!-- http://geographicknowledge.de/vocab/CoreConceptData.rdf#AmountDS -->

    <owl:Class rdf:about="http://geographicknowledge.de/vocab/CoreConceptData.rdf#AmountDS">
        <rdfs:subClassOf rdf:resource="http://geographicknowledge.de/vocab/CoreConceptData.rdf#CoreConceptDataSet"/>
        <rdfs:comment xml:lang="en">Dataset of amounts of objects</rdfs:comment>
    </owl:Class>
    


    <!-- http://geographicknowledge.de/vocab/CoreConceptData.rdf#AmountRasterDS -->

    <owl:Class rdf:about="http://geographicknowledge.de/vocab/CoreConceptData.rdf#AmountRasterDS">
        <owl:equivalentClass>
            <owl:Class>
                <owl:intersectionOf rdf:parseType="Collection">
                    <rdf:Description rdf:about="http://geographicknowledge.de/vocab/CoreConceptData.rdf#AmountDS"/>
                    <rdf:Description rdf:about="http://geographicknowledge.de/vocab/CoreConceptData.rdf#Raster"/>
                </owl:intersectionOf>
            </owl:Class>
        </owl:equivalentClass>
        <rdfs:subClassOf rdf:resource="http://geographicknowledge.de/vocab/CoreConceptData.rdf#AmountDS"/>
        <rdfs:comment xml:lang="en">A raster data set where each cell represents an amount of objects</rdfs:comment>
    </owl:Class>
    


    <!-- http://geographicknowledge.de/vocab/CoreConceptData.rdf#AmountVectorDS -->

    <owl:Class rdf:about="http://geographicknowledge.de/vocab/CoreConceptData.rdf#AmountVectorDS">
        <owl:equivalentClass>
            <owl:Class>
                <owl:intersectionOf rdf:parseType="Collection">
                    <rdf:Description rdf:about="http://geographicknowledge.de/vocab/CoreConceptData.rdf#AmountDS"/>
                    <rdf:Description rdf:about="http://geographicknowledge.de/vocab/CoreConceptData.rdf#Vector"/>
                </owl:intersectionOf>
            </owl:Class>
        </owl:equivalentClass>
        <rdfs:subClassOf rdf:resource="http://geographicknowledge.de/vocab/CoreConceptData.rdf#AmountDS"/>
        <rdfs:comment xml:lang="en">A dataset where each geometry denotes an amount of objects</rdfs:comment>
    </owl:Class>
    


    <!-- http://geographicknowledge.de/vocab/CoreConceptData.rdf#Attribute -->

    <owl:Class rdf:about="http://geographicknowledge.de/vocab/CoreConceptData.rdf#Attribute">
        <rdfs:subClassOf rdf:resource="http://geographicknowledge.de/vocab/AnalysisData.rdf#ValueList"/>
        <rdfs:comment xml:lang="en">Attributes of a tabular dataset. Each attribute corresponds to a column in the table.</rdfs:comment>
    </owl:Class>
    


    <!-- http://geographicknowledge.de/vocab/CoreConceptData.rdf#BooleanA -->

    <owl:Class rdf:about="http://geographicknowledge.de/vocab/CoreConceptData.rdf#BooleanA">
        <rdfs:subClassOf rdf:resource="http://geographicknowledge.de/vocab/CoreConceptData.rdf#NominalA"/>
        <rdfs:comment xml:lang="en">Boolean attributes are spatial attributes within the range of True/False. They are special types of (bi)nominal attributes</rdfs:comment>
    </owl:Class>
    


    <!-- http://geographicknowledge.de/vocab/CoreConceptData.rdf#BoundedPhen -->

    <owl:Class rdf:about="http://geographicknowledge.de/vocab/CoreConceptData.rdf#BoundedPhen">
        <owl:equivalentClass>
            <owl:Class>
                <owl:unionOf rdf:parseType="Collection">
                    <rdf:Description rdf:about="http://geographicknowledge.de/vocab/CoreConceptData.rdf#ExistenceRaster"/>
                    <rdf:Description rdf:about="http://geographicknowledge.de/vocab/CoreConceptData.rdf#ExistenceVector"/>
                    <rdf:Description rdf:about="http://geographicknowledge.de/vocab/CoreConceptData.rdf#ObjectVector"/>
                </owl:unionOf>
            </owl:Class>
        </owl:equivalentClass>
        <rdfs:subClassOf rdf:resource="http://geographicknowledge.de/vocab/CoreConceptData.rdf#Attribute"/>
        <rdfs:comment xml:lang="en">This is a spatial attribute which denotes a bounded phenomenon. Can be either a object vector or an existence raster</rdfs:comment>
    </owl:Class>
    


    <!-- http://geographicknowledge.de/vocab/CoreConceptData.rdf#Contour -->

    <owl:Class rdf:about="http://geographicknowledge.de/vocab/CoreConceptData.rdf#Contour">
        <rdfs:subClassOf rdf:resource="http://geographicknowledge.de/vocab/CoreConceptData.rdf#Coverage"/>
        <rdfs:subClassOf rdf:resource="http://geographicknowledge.de/vocab/CoreConceptData.rdf#OrdinalA"/>
        <rdfs:comment xml:lang="en">Contour layers are coverages that denote intervals of the reprepresented continuous field. For example, temperature intervals, represented as regions bounded by isolines of a temperature field.</rdfs:comment>
    </owl:Class>
    


    <!-- http://geographicknowledge.de/vocab/CoreConceptData.rdf#ContourDS -->

    <owl:Class rdf:about="http://geographicknowledge.de/vocab/CoreConceptData.rdf#ContourDS">
        <rdfs:subClassOf rdf:resource="http://geographicknowledge.de/vocab/CoreConceptData.rdf#CoverageDS"/>
        <rdfs:comment xml:lang="en">A dataset representing a field using contours, which denote the boundaries of value intervals. For example, a terrain contour map.</rdfs:comment>
    </owl:Class>
    


    <!-- http://geographicknowledge.de/vocab/CoreConceptData.rdf#CoreConceptDataSet -->

    <owl:Class rdf:about="http://geographicknowledge.de/vocab/CoreConceptData.rdf#CoreConceptDataSet">
        <rdfs:subClassOf rdf:resource="http://geographicknowledge.de/vocab/AnalysisData.rdf#SpatialDataSet"/>
        <rdfs:comment xml:lang="en">A data set which represents a core concept of spatial information. The attributes of this dataset are assumed to be of corresponding types.</rdfs:comment>
    </owl:Class>
    


    <!-- http://geographicknowledge.de/vocab/CoreConceptData.rdf#CountA -->

    <owl:Class rdf:about="http://geographicknowledge.de/vocab/CoreConceptData.rdf#CountA">
        <rdfs:subClassOf rdf:resource="http://geographicknowledge.de/vocab/CoreConceptData.rdf#RatioA"/>
        <rdfs:comment xml:lang="en">An attribute that denotes counts of discrete entities (compare Chrisman 1998)</rdfs:comment>
    </owl:Class>
    


    <!-- http://geographicknowledge.de/vocab/CoreConceptData.rdf#Coverage -->

    <owl:Class rdf:about="http://geographicknowledge.de/vocab/CoreConceptData.rdf#Coverage">
        <owl:equivalentClass>
            <owl:Class>
                <owl:intersectionOf rdf:parseType="Collection">
                    <rdf:Description rdf:about="http://geographicknowledge.de/vocab/CoreConceptData.rdf#FieldQ"/>
                    <owl:Restriction>
                        <owl:onProperty rdf:resource="http://geographicknowledge.de/vocab/AnalysisData.rdf#ofDataSet"/>
                        <owl:someValuesFrom rdf:resource="http://geographicknowledge.de/vocab/CoreConceptData.rdf#Tessellation"/>
                    </owl:Restriction>
                </owl:intersectionOf>
            </owl:Class>
        </owl:equivalentClass>
        <rdfs:subClassOf rdf:resource="http://geographicknowledge.de/vocab/CoreConceptData.rdf#TessellationA"/>
        <rdfs:comment xml:lang="en">Coverages are tessellated layers that represent a continuous field. For example, landuse polygons.</rdfs:comment>
    </owl:Class>
    


    <!-- http://geographicknowledge.de/vocab/CoreConceptData.rdf#CoverageDS -->

    <owl:Class rdf:about="http://geographicknowledge.de/vocab/CoreConceptData.rdf#CoverageDS">
        <owl:equivalentClass>
            <owl:Class>
                <owl:intersectionOf rdf:parseType="Collection">
                    <rdf:Description rdf:about="http://geographicknowledge.de/vocab/CoreConceptData.rdf#FieldDS"/>
                    <rdf:Description rdf:about="http://geographicknowledge.de/vocab/CoreConceptData.rdf#Tessellation"/>
                </owl:intersectionOf>
            </owl:Class>
        </owl:equivalentClass>
        <rdfs:subClassOf rdf:resource="http://geographicknowledge.de/vocab/CoreConceptData.rdf#FieldDS"/>
        <rdfs:comment xml:lang="en">A dataset representing a field using (possibly irregular) patches of homogeneous values. For example, a landuse map or a soil map.</rdfs:comment>
    </owl:Class>
    


    <!-- http://geographicknowledge.de/vocab/CoreConceptData.rdf#EventDS -->

    <owl:Class rdf:about="http://geographicknowledge.de/vocab/CoreConceptData.rdf#EventDS">
        <rdfs:subClassOf rdf:resource="http://geographicknowledge.de/vocab/CoreConceptData.rdf#CoreConceptDataSet"/>
        <rdfs:comment xml:lang="en">A spatial dataset representing events</rdfs:comment>
    </owl:Class>
    


    <!-- http://geographicknowledge.de/vocab/CoreConceptData.rdf#EventQ -->

    <owl:Class rdf:about="http://geographicknowledge.de/vocab/CoreConceptData.rdf#EventQ">
        <owl:equivalentClass>
            <owl:Restriction>
                <owl:onProperty rdf:resource="http://geographicknowledge.de/vocab/AnalysisData.rdf#ofDataSet"/>
                <owl:someValuesFrom rdf:resource="http://geographicknowledge.de/vocab/CoreConceptData.rdf#EventDS"/>
            </owl:Restriction>
        </owl:equivalentClass>
        <rdfs:subClassOf rdf:resource="http://geographicknowledge.de/vocab/CoreConceptData.rdf#Attribute"/>
        <rdfs:comment xml:lang="en">This attribute represents a quality of an event (core concept). For example, the duration.</rdfs:comment>
    </owl:Class>
    


    <!-- http://geographicknowledge.de/vocab/CoreConceptData.rdf#EventVector -->

    <owl:Class rdf:about="http://geographicknowledge.de/vocab/CoreConceptData.rdf#EventVector">
        <owl:equivalentClass>
            <owl:Class>
                <owl:intersectionOf rdf:parseType="Collection">
                    <rdf:Description rdf:about="http://geographicknowledge.de/vocab/CoreConceptData.rdf#EventQ"/>
                    <owl:Restriction>
                        <owl:onProperty rdf:resource="http://geographicknowledge.de/vocab/AnalysisData.rdf#ofDataSet"/>
                        <owl:someValuesFrom rdf:resource="http://geographicknowledge.de/vocab/CoreConceptData.rdf#Vector"/>
                    </owl:Restriction>
                </owl:intersectionOf>
            </owl:Class>
        </owl:equivalentClass>
        <rdfs:subClassOf rdf:resource="http://geographicknowledge.de/vocab/CoreConceptData.rdf#VectorA"/>
        <rdfs:comment xml:lang="en">Events represented in terms of an attribute of a vector data set. For example, the magnitude of earthquakes represented as an attribute of a point data set.</rdfs:comment>
    </owl:Class>
    


    <!-- http://geographicknowledge.de/vocab/CoreConceptData.rdf#ExistenceRaster -->

    <owl:Class rdf:about="http://geographicknowledge.de/vocab/CoreConceptData.rdf#ExistenceRaster">
        <owl:equivalentClass>
            <owl:Class>
                <owl:intersectionOf rdf:parseType="Collection">
                    <rdf:Description rdf:about="http://geographicknowledge.de/vocab/CoreConceptData.rdf#BooleanA"/>
                    <rdf:Description rdf:about="http://geographicknowledge.de/vocab/CoreConceptData.rdf#FieldRaster"/>
                </owl:intersectionOf>
            </owl:Class>
        </owl:equivalentClass>
        <rdfs:comment xml:lang="en">Existence rasters are rasters representing boolean fields (fields denoting whether something is present at a cell location or not).</rdfs:comment>
    </owl:Class>
    


    <!-- http://geographicknowledge.de/vocab/CoreConceptData.rdf#ExistenceVector -->

    <owl:Class rdf:about="http://geographicknowledge.de/vocab/CoreConceptData.rdf#ExistenceVector">
        <owl:equivalentClass>
            <owl:Class>
                <owl:intersectionOf rdf:parseType="Collection">
                    <rdf:Description rdf:about="http://geographicknowledge.de/vocab/CoreConceptData.rdf#BooleanA"/>
                    <rdf:Description rdf:about="http://geographicknowledge.de/vocab/CoreConceptData.rdf#FieldVector"/>
                </owl:intersectionOf>
            </owl:Class>
        </owl:equivalentClass>
        <rdfs:subClassOf rdf:resource="http://geographicknowledge.de/vocab/CoreConceptData.rdf#VectorA"/>
        <rdfs:comment xml:lang="en">A vector layer attribute that satisfies a boolean expression and thus denotes the &apos;existence&apos; of some attribute encoded phenomenon across space. Example is a layer of polygons of &apos;&apos;forest&apos;&apos; landuse or a layer of &quot;parks&quot;.</rdfs:comment>
    </owl:Class>
    


    <!-- http://geographicknowledge.de/vocab/CoreConceptData.rdf#ExtLattice -->

    <owl:Class rdf:about="http://geographicknowledge.de/vocab/CoreConceptData.rdf#ExtLattice">
        <owl:equivalentClass>
            <owl:Class>
                <owl:intersectionOf rdf:parseType="Collection">
                    <rdf:Description rdf:about="http://geographicknowledge.de/vocab/CoreConceptData.rdf#Lattice"/>
                    <rdf:Description rdf:about="http://geographicknowledge.de/vocab/ExtensiveMeasures.rdf#ERA"/>
                </owl:intersectionOf>
            </owl:Class>
        </owl:equivalentClass>
        <rdfs:comment xml:lang="en">This type of lattice has an extensive attribute. For example, a spatial dataset about the population number of municipalities</rdfs:comment>
    </owl:Class>
    


    <!-- http://geographicknowledge.de/vocab/CoreConceptData.rdf#FieldDS -->

    <owl:Class rdf:about="http://geographicknowledge.de/vocab/CoreConceptData.rdf#FieldDS">
        <rdfs:subClassOf rdf:resource="http://geographicknowledge.de/vocab/CoreConceptData.rdf#CoreConceptDataSet"/>
        <rdfs:comment xml:lang="en">A spatial dataset representing a field</rdfs:comment>
    </owl:Class>
    


    <!-- http://geographicknowledge.de/vocab/CoreConceptData.rdf#FieldQ -->

    <owl:Class rdf:about="http://geographicknowledge.de/vocab/CoreConceptData.rdf#FieldQ">
        <owl:equivalentClass>
            <owl:Restriction>
                <owl:onProperty rdf:resource="http://geographicknowledge.de/vocab/AnalysisData.rdf#ofDataSet"/>
                <owl:someValuesFrom rdf:resource="http://geographicknowledge.de/vocab/CoreConceptData.rdf#FieldDS"/>
            </owl:Restriction>
        </owl:equivalentClass>
        <rdfs:subClassOf rdf:resource="http://geographicknowledge.de/vocab/CoreConceptData.rdf#Attribute"/>
        <rdfs:comment xml:lang="en">An attribute which represents the quality of a field (core concept). This implies that the spatial data items in this data set are self-similar (their parts have the same attribute)</rdfs:comment>
    </owl:Class>
    


    <!-- http://geographicknowledge.de/vocab/CoreConceptData.rdf#FieldRaster -->

    <owl:Class rdf:about="http://geographicknowledge.de/vocab/CoreConceptData.rdf#FieldRaster">
        <owl:equivalentClass>
            <owl:Class>
                <owl:intersectionOf rdf:parseType="Collection">
                    <rdf:Description rdf:about="http://geographicknowledge.de/vocab/CoreConceptData.rdf#FieldQ"/>
                    <owl:Restriction>
                        <owl:onProperty rdf:resource="http://geographicknowledge.de/vocab/AnalysisData.rdf#ofDataSet"/>
                        <owl:someValuesFrom rdf:resource="http://geographicknowledge.de/vocab/CoreConceptData.rdf#Raster"/>
                    </owl:Restriction>
                </owl:intersectionOf>
            </owl:Class>
        </owl:equivalentClass>
        <rdfs:subClassOf rdf:resource="http://geographicknowledge.de/vocab/CoreConceptData.rdf#RasterA"/>
        <rdfs:comment xml:lang="en">Field rasters are raster representations of continuous fields. For example, raster layers representing a terrain height (DTM).</rdfs:comment>
    </owl:Class>
    


    <!-- http://geographicknowledge.de/vocab/CoreConceptData.rdf#FieldRasterDS -->

    <owl:Class rdf:about="http://geographicknowledge.de/vocab/CoreConceptData.rdf#FieldRasterDS">
        <owl:equivalentClass>
            <owl:Class>
                <owl:intersectionOf rdf:parseType="Collection">
                    <rdf:Description rdf:about="http://geographicknowledge.de/vocab/CoreConceptData.rdf#FieldDS"/>
                    <rdf:Description rdf:about="http://geographicknowledge.de/vocab/CoreConceptData.rdf#Raster"/>
                </owl:intersectionOf>
            </owl:Class>
        </owl:equivalentClass>
        <rdfs:subClassOf rdf:resource="http://geographicknowledge.de/vocab/CoreConceptData.rdf#FieldDS"/>
        <rdfs:comment xml:lang="en">A dataset representing a field by homogeneous values using raster cells</rdfs:comment>
    </owl:Class>
    


    <!-- http://geographicknowledge.de/vocab/CoreConceptData.rdf#FieldVector -->

    <owl:Class rdf:about="http://geographicknowledge.de/vocab/CoreConceptData.rdf#FieldVector">
        <owl:equivalentClass>
            <owl:Class>
                <owl:intersectionOf rdf:parseType="Collection">
                    <rdf:Description rdf:about="http://geographicknowledge.de/vocab/CoreConceptData.rdf#FieldQ"/>
                    <owl:Restriction>
                        <owl:onProperty rdf:resource="http://geographicknowledge.de/vocab/AnalysisData.rdf#ofDataSet"/>
                        <owl:someValuesFrom rdf:resource="http://geographicknowledge.de/vocab/CoreConceptData.rdf#Vector"/>
                    </owl:Restriction>
                </owl:intersectionOf>
            </owl:Class>
        </owl:equivalentClass>
        <rdfs:subClassOf rdf:resource="http://geographicknowledge.de/vocab/CoreConceptData.rdf#VectorA"/>
        <rdfs:comment xml:lang="en">A vector representation of a field. Can be a point or line measure, or a coverage</rdfs:comment>
    </owl:Class>
    


    <!-- http://geographicknowledge.de/vocab/CoreConceptData.rdf#IntervalA -->

    <owl:Class rdf:about="http://geographicknowledge.de/vocab/CoreConceptData.rdf#IntervalA">
        <rdfs:subClassOf rdf:resource="http://geographicknowledge.de/vocab/CoreConceptData.rdf#OrdinalA"/>
        <rdfs:comment xml:lang="en">An interval scaled attribute</rdfs:comment>
    </owl:Class>
    


    <!-- http://geographicknowledge.de/vocab/CoreConceptData.rdf#Lattice -->

    <owl:Class rdf:about="http://geographicknowledge.de/vocab/CoreConceptData.rdf#Lattice">
        <owl:equivalentClass>
            <owl:Class>
                <owl:intersectionOf rdf:parseType="Collection">
                    <rdf:Description rdf:about="http://geographicknowledge.de/vocab/CoreConceptData.rdf#ObjectQ"/>
                    <owl:Restriction>
                        <owl:onProperty rdf:resource="http://geographicknowledge.de/vocab/AnalysisData.rdf#ofDataSet"/>
                        <owl:someValuesFrom rdf:resource="http://geographicknowledge.de/vocab/CoreConceptData.rdf#Tessellation"/>
                    </owl:Restriction>
                </owl:intersectionOf>
            </owl:Class>
        </owl:equivalentClass>
        <rdfs:subClassOf rdf:resource="http://geographicknowledge.de/vocab/CoreConceptData.rdf#TessellationA"/>
        <rdfs:comment xml:lang="en">A lattice is a spatial tessellation that represents objects and their qualities. For example, a set of municipalities with average income.</rdfs:comment>
    </owl:Class>
    


    <!-- http://geographicknowledge.de/vocab/CoreConceptData.rdf#LatticeDS -->

    <owl:Class rdf:about="http://geographicknowledge.de/vocab/CoreConceptData.rdf#LatticeDS">
        <owl:equivalentClass>
            <owl:Class>
                <owl:intersectionOf rdf:parseType="Collection">
                    <rdf:Description rdf:about="http://geographicknowledge.de/vocab/CoreConceptData.rdf#ObjectDS"/>
                    <rdf:Description rdf:about="http://geographicknowledge.de/vocab/CoreConceptData.rdf#Tessellation"/>
                </owl:intersectionOf>
            </owl:Class>
        </owl:equivalentClass>
        <rdfs:subClassOf rdf:resource="http://geographicknowledge.de/vocab/CoreConceptData.rdf#ObjectDS"/>
        <rdfs:comment xml:lang="en">A dataset of objects which tesselate space and contain statistical summaries. For example, the municipalities of the Netherlands</rdfs:comment>
    </owl:Class>
    


    <!-- http://geographicknowledge.de/vocab/CoreConceptData.rdf#Line -->

    <owl:Class rdf:about="http://geographicknowledge.de/vocab/CoreConceptData.rdf#Line">
        <rdfs:subClassOf rdf:resource="http://geographicknowledge.de/vocab/AnalysisData.rdf#Spatial"/>
        <rdfs:comment xml:lang="en">A generalized notion of a line in 2D and 3D</rdfs:comment>
    </owl:Class>
    


    <!-- http://geographicknowledge.de/vocab/CoreConceptData.rdf#LineA -->

    <owl:Class rdf:about="http://geographicknowledge.de/vocab/CoreConceptData.rdf#LineA">
        <owl:equivalentClass>
            <owl:Class>
                <owl:intersectionOf rdf:parseType="Collection">
                    <rdf:Description rdf:about="http://geographicknowledge.de/vocab/CoreConceptData.rdf#Attribute"/>
                    <owl:Restriction>
                        <owl:onProperty rdf:resource="http://geographicknowledge.de/vocab/AnalysisData.rdf#ofDataSet"/>
                        <owl:someValuesFrom rdf:resource="http://geographicknowledge.de/vocab/CoreConceptData.rdf#LineDataSet"/>
                    </owl:Restriction>
                </owl:intersectionOf>
            </owl:Class>
        </owl:equivalentClass>
        <rdfs:subClassOf rdf:resource="http://geographicknowledge.de/vocab/CoreConceptData.rdf#Attribute"/>
        <rdfs:subClassOf rdf:resource="http://geographicknowledge.de/vocab/CoreConceptData.rdf#VectorA"/>
        <rdfs:comment xml:lang="en">Attribute of some Line data set</rdfs:comment>
    </owl:Class>
    


    <!-- http://geographicknowledge.de/vocab/CoreConceptData.rdf#LineData -->

    <owl:Class rdf:about="http://geographicknowledge.de/vocab/CoreConceptData.rdf#LineData">
        <owl:equivalentClass>
            <owl:Class>
                <owl:intersectionOf rdf:parseType="Collection">
                    <rdf:Description rdf:about="http://geographicknowledge.de/vocab/AnalysisData.rdf#SpatialData"/>
                    <owl:Restriction>
                        <owl:onProperty rdf:resource="http://geographicknowledge.de/vocab/GISConcepts.rdf#hasAttribute"/>
                        <owl:someValuesFrom rdf:resource="http://geographicknowledge.de/vocab/CoreConceptData.rdf#Line"/>
                    </owl:Restriction>
                </owl:intersectionOf>
            </owl:Class>
        </owl:equivalentClass>
    </owl:Class>
    


    <!-- http://geographicknowledge.de/vocab/CoreConceptData.rdf#LineDataSet -->

    <owl:Class rdf:about="http://geographicknowledge.de/vocab/CoreConceptData.rdf#LineDataSet">
        <owl:equivalentClass>
            <owl:Class>
                <owl:intersectionOf rdf:parseType="Collection">
                    <rdf:Description rdf:about="http://geographicknowledge.de/vocab/CoreConceptData.rdf#Vector"/>
                    <owl:Restriction>
                        <owl:onProperty rdf:resource="http://geographicknowledge.de/vocab/AnalysisData.rdf#hasElement"/>
                        <owl:allValuesFrom rdf:resource="http://geographicknowledge.de/vocab/CoreConceptData.rdf#LineData"/>
                    </owl:Restriction>
                </owl:intersectionOf>
            </owl:Class>
        </owl:equivalentClass>
        <owl:disjointWith rdf:resource="http://geographicknowledge.de/vocab/CoreConceptData.rdf#PointDataSet"/>
        <owl:disjointWith rdf:resource="http://geographicknowledge.de/vocab/CoreConceptData.rdf#RegionDataSet"/>
    </owl:Class>
    


    <!-- http://geographicknowledge.de/vocab/CoreConceptData.rdf#LineMeasures -->

    <owl:Class rdf:about="http://geographicknowledge.de/vocab/CoreConceptData.rdf#LineMeasures">
        <owl:equivalentClass>
            <owl:Class>
                <owl:intersectionOf rdf:parseType="Collection">
                    <rdf:Description rdf:about="http://geographicknowledge.de/vocab/CoreConceptData.rdf#FieldQ"/>
                    <owl:Restriction>
                        <owl:onProperty rdf:resource="http://geographicknowledge.de/vocab/AnalysisData.rdf#ofDataSet"/>
                        <owl:someValuesFrom rdf:resource="http://geographicknowledge.de/vocab/CoreConceptData.rdf#LineDataSet"/>
                    </owl:Restriction>
                </owl:intersectionOf>
            </owl:Class>
        </owl:equivalentClass>
        <rdfs:subClassOf rdf:resource="http://geographicknowledge.de/vocab/CoreConceptData.rdf#FieldVector"/>
        <rdfs:subClassOf rdf:resource="http://geographicknowledge.de/vocab/CoreConceptData.rdf#LineA"/>
        <rdfs:comment xml:lang="en">Linear representations of fields. Examples are isoline maps</rdfs:comment>
    </owl:Class>
    


    <!-- http://geographicknowledge.de/vocab/CoreConceptData.rdf#LineMeasuresDS -->

    <owl:Class rdf:about="http://geographicknowledge.de/vocab/CoreConceptData.rdf#LineMeasuresDS">
        <owl:equivalentClass>
            <owl:Class>
                <owl:intersectionOf rdf:parseType="Collection">
                    <rdf:Description rdf:about="http://geographicknowledge.de/vocab/CoreConceptData.rdf#FieldDS"/>
                    <rdf:Description rdf:about="http://geographicknowledge.de/vocab/CoreConceptData.rdf#LineDataSet"/>
                </owl:intersectionOf>
            </owl:Class>
        </owl:equivalentClass>
        <rdfs:subClassOf rdf:resource="http://geographicknowledge.de/vocab/CoreConceptData.rdf#FieldDS"/>
        <rdfs:comment xml:lang="en">A representation of a field as a line of homogeneous values</rdfs:comment>
    </owl:Class>
    


    <!-- http://geographicknowledge.de/vocab/CoreConceptData.rdf#NetworkDS -->

    <owl:Class rdf:about="http://geographicknowledge.de/vocab/CoreConceptData.rdf#NetworkDS">
        <rdfs:subClassOf rdf:resource="http://geographicknowledge.de/vocab/CoreConceptData.rdf#CoreConceptDataSet"/>
        <rdfs:comment xml:lang="en">A spatial dataset representing a spatial network. Note thate a network in the sense of a core concept is a quantified relation between objects. For example, the traffic flow between municipalities or between two intersections. Streets themselves can also be seen as objects if they do not encode such relations</rdfs:comment>
    </owl:Class>
    


    <!-- http://geographicknowledge.de/vocab/CoreConceptData.rdf#NetworkQ -->

    <owl:Class rdf:about="http://geographicknowledge.de/vocab/CoreConceptData.rdf#NetworkQ">
        <owl:equivalentClass>
            <owl:Restriction>
                <owl:onProperty rdf:resource="http://geographicknowledge.de/vocab/AnalysisData.rdf#ofDataSet"/>
                <owl:someValuesFrom rdf:resource="http://geographicknowledge.de/vocab/CoreConceptData.rdf#NetworkDS"/>
            </owl:Restriction>
        </owl:equivalentClass>
        <rdfs:subClassOf rdf:resource="http://geographicknowledge.de/vocab/CoreConceptData.rdf#Attribute"/>
        <rdfs:comment xml:lang="en">This attribute represents the quality of a network edge.</rdfs:comment>
    </owl:Class>
    


    <!-- http://geographicknowledge.de/vocab/CoreConceptData.rdf#NoDataExistenceRaster -->

    <owl:Class rdf:about="http://geographicknowledge.de/vocab/CoreConceptData.rdf#NoDataExistenceRaster">
        <rdfs:subClassOf rdf:resource="http://geographicknowledge.de/vocab/CoreConceptData.rdf#ExistenceRaster"/>
        <rdfs:comment xml:lang="en">A raster dataset where  NoData is interpreted as boolean &quot;false&quot;.</rdfs:comment>
    </owl:Class>
    


    <!-- http://geographicknowledge.de/vocab/CoreConceptData.rdf#NominalA -->

    <owl:Class rdf:about="http://geographicknowledge.de/vocab/CoreConceptData.rdf#NominalA">
        <rdfs:subClassOf rdf:resource="http://geographicknowledge.de/vocab/CoreConceptData.rdf#Attribute"/>
        <rdfs:comment xml:lang="en">A spatial attribute on nominal scale level</rdfs:comment>
    </owl:Class>
    


    <!-- http://geographicknowledge.de/vocab/CoreConceptData.rdf#ObjectDS -->

    <owl:Class rdf:about="http://geographicknowledge.de/vocab/CoreConceptData.rdf#ObjectDS">
        <rdfs:subClassOf rdf:resource="http://geographicknowledge.de/vocab/CoreConceptData.rdf#CoreConceptDataSet"/>
        <rdfs:comment xml:lang="en">A spatial data set representing objects</rdfs:comment>
    </owl:Class>
    


    <!-- http://geographicknowledge.de/vocab/CoreConceptData.rdf#ObjectLine -->

    <owl:Class rdf:about="http://geographicknowledge.de/vocab/CoreConceptData.rdf#ObjectLine">
        <owl:equivalentClass>
            <owl:Class>
                <owl:intersectionOf rdf:parseType="Collection">
                    <rdf:Description rdf:about="http://geographicknowledge.de/vocab/CoreConceptData.rdf#ObjectQ"/>
                    <owl:Restriction>
                        <owl:onProperty rdf:resource="http://geographicknowledge.de/vocab/AnalysisData.rdf#ofDataSet"/>
                        <owl:someValuesFrom rdf:resource="http://geographicknowledge.de/vocab/CoreConceptData.rdf#LineDataSet"/>
                    </owl:Restriction>
                </owl:intersectionOf>
            </owl:Class>
        </owl:equivalentClass>
        <rdfs:subClassOf rdf:resource="http://geographicknowledge.de/vocab/CoreConceptData.rdf#LineA"/>
        <rdfs:subClassOf rdf:resource="http://geographicknowledge.de/vocab/CoreConceptData.rdf#ObjectVector"/>
        <rdfs:comment xml:lang="en">An attribute of an object line dataset</rdfs:comment>
    </owl:Class>
    


    <!-- http://geographicknowledge.de/vocab/CoreConceptData.rdf#ObjectPoint -->

    <owl:Class rdf:about="http://geographicknowledge.de/vocab/CoreConceptData.rdf#ObjectPoint">
        <owl:equivalentClass>
            <owl:Class>
                <owl:intersectionOf rdf:parseType="Collection">
                    <rdf:Description rdf:about="http://geographicknowledge.de/vocab/CoreConceptData.rdf#ObjectQ"/>
                    <owl:Restriction>
                        <owl:onProperty rdf:resource="http://geographicknowledge.de/vocab/AnalysisData.rdf#ofDataSet"/>
                        <owl:someValuesFrom rdf:resource="http://geographicknowledge.de/vocab/CoreConceptData.rdf#PointDataSet"/>
                    </owl:Restriction>
                </owl:intersectionOf>
            </owl:Class>
        </owl:equivalentClass>
        <rdfs:subClassOf rdf:resource="http://geographicknowledge.de/vocab/CoreConceptData.rdf#ObjectVector"/>
        <rdfs:subClassOf rdf:resource="http://geographicknowledge.de/vocab/CoreConceptData.rdf#PointA"/>
        <rdfs:comment xml:lang="en">An attribute of an object point dataset</rdfs:comment>
    </owl:Class>
    


    <!-- http://geographicknowledge.de/vocab/CoreConceptData.rdf#ObjectQ -->

    <owl:Class rdf:about="http://geographicknowledge.de/vocab/CoreConceptData.rdf#ObjectQ">
        <owl:equivalentClass>
            <owl:Restriction>
                <owl:onProperty rdf:resource="http://geographicknowledge.de/vocab/AnalysisData.rdf#ofDataSet"/>
                <owl:someValuesFrom rdf:resource="http://geographicknowledge.de/vocab/CoreConceptData.rdf#ObjectDS"/>
            </owl:Restriction>
        </owl:equivalentClass>
        <rdfs:subClassOf rdf:resource="http://geographicknowledge.de/vocab/CoreConceptData.rdf#Attribute"/>
        <rdfs:comment xml:lang="en">An attribute that represents the quality of an object (core concept)</rdfs:comment>
    </owl:Class>
    


    <!-- http://geographicknowledge.de/vocab/CoreConceptData.rdf#ObjectRegion -->

    <owl:Class rdf:about="http://geographicknowledge.de/vocab/CoreConceptData.rdf#ObjectRegion">
        <owl:equivalentClass>
            <owl:Class>
                <owl:intersectionOf rdf:parseType="Collection">
                    <rdf:Description rdf:about="http://geographicknowledge.de/vocab/CoreConceptData.rdf#ObjectQ"/>
                    <owl:Restriction>
                        <owl:onProperty rdf:resource="http://geographicknowledge.de/vocab/AnalysisData.rdf#ofDataSet"/>
                        <owl:someValuesFrom rdf:resource="http://geographicknowledge.de/vocab/CoreConceptData.rdf#RegionDataSet"/>
                    </owl:Restriction>
                </owl:intersectionOf>
            </owl:Class>
        </owl:equivalentClass>
        <rdfs:subClassOf rdf:resource="http://geographicknowledge.de/vocab/CoreConceptData.rdf#ObjectVector"/>
        <rdfs:subClassOf rdf:resource="http://geographicknowledge.de/vocab/CoreConceptData.rdf#RegionA"/>
    </owl:Class>
    


    <!-- http://geographicknowledge.de/vocab/CoreConceptData.rdf#ObjectVector -->

    <owl:Class rdf:about="http://geographicknowledge.de/vocab/CoreConceptData.rdf#ObjectVector">
        <owl:equivalentClass>
            <owl:Class>
                <owl:intersectionOf rdf:parseType="Collection">
                    <rdf:Description rdf:about="http://geographicknowledge.de/vocab/CoreConceptData.rdf#ObjectQ"/>
                    <owl:Restriction>
                        <owl:onProperty rdf:resource="http://geographicknowledge.de/vocab/AnalysisData.rdf#ofDataSet"/>
                        <owl:someValuesFrom rdf:resource="http://geographicknowledge.de/vocab/CoreConceptData.rdf#Vector"/>
                    </owl:Restriction>
                </owl:intersectionOf>
            </owl:Class>
        </owl:equivalentClass>
        <rdfs:subClassOf rdf:resource="http://geographicknowledge.de/vocab/CoreConceptData.rdf#Attribute"/>
        <rdfs:subClassOf rdf:resource="http://geographicknowledge.de/vocab/CoreConceptData.rdf#VectorA"/>
        <rdfs:comment xml:lang="en">Object vectors are vector representation of a set of objecs and their quality. For example, a point layer denoting points of Interest (POI) or buildings in a city together with their quality, e.g. the building height.</rdfs:comment>
    </owl:Class>
    


    <!-- http://geographicknowledge.de/vocab/CoreConceptData.rdf#OrdinalA -->

    <owl:Class rdf:about="http://geographicknowledge.de/vocab/CoreConceptData.rdf#OrdinalA">
        <rdfs:subClassOf rdf:resource="http://geographicknowledge.de/vocab/CoreConceptData.rdf#NominalA"/>
        <rdfs:comment xml:lang="en">A spatial attribute on ordinal scale level</rdfs:comment>
    </owl:Class>
    


    <!-- http://geographicknowledge.de/vocab/CoreConceptData.rdf#PatchDS -->

    <owl:Class rdf:about="http://geographicknowledge.de/vocab/CoreConceptData.rdf#PatchDS">
        <owl:equivalentClass>
            <owl:Class>
                <owl:intersectionOf rdf:parseType="Collection">
                    <rdf:Description rdf:about="http://geographicknowledge.de/vocab/CoreConceptData.rdf#FieldDS"/>
                    <rdf:Description rdf:about="http://geographicknowledge.de/vocab/CoreConceptData.rdf#RegionDataSet"/>
                </owl:intersectionOf>
            </owl:Class>
        </owl:equivalentClass>
        <rdfs:subClassOf rdf:resource="http://geographicknowledge.de/vocab/CoreConceptData.rdf#FieldDS"/>
        <rdfs:comment xml:lang="en">A dataset which represents a field in terms patches of homogeneous values. Not necessarily tessellated</rdfs:comment>
    </owl:Class>
    


    <!-- http://geographicknowledge.de/vocab/CoreConceptData.rdf#Point -->

    <owl:Class rdf:about="http://geographicknowledge.de/vocab/CoreConceptData.rdf#Point">
        <rdfs:subClassOf rdf:resource="http://geographicknowledge.de/vocab/AnalysisData.rdf#Spatial"/>
        <rdfs:comment xml:lang="en">A generalized notion of a point in 2D and 3D</rdfs:comment>
    </owl:Class>
    


    <!-- http://geographicknowledge.de/vocab/CoreConceptData.rdf#PointA -->

    <owl:Class rdf:about="http://geographicknowledge.de/vocab/CoreConceptData.rdf#PointA">
        <owl:equivalentClass>
            <owl:Class>
                <owl:intersectionOf rdf:parseType="Collection">
                    <rdf:Description rdf:about="http://geographicknowledge.de/vocab/CoreConceptData.rdf#Attribute"/>
                    <owl:Restriction>
                        <owl:onProperty rdf:resource="http://geographicknowledge.de/vocab/AnalysisData.rdf#ofDataSet"/>
                        <owl:someValuesFrom rdf:resource="http://geographicknowledge.de/vocab/CoreConceptData.rdf#PointDataSet"/>
                    </owl:Restriction>
                </owl:intersectionOf>
            </owl:Class>
        </owl:equivalentClass>
        <rdfs:subClassOf rdf:resource="http://geographicknowledge.de/vocab/CoreConceptData.rdf#Attribute"/>
        <rdfs:subClassOf rdf:resource="http://geographicknowledge.de/vocab/CoreConceptData.rdf#VectorA"/>
        <rdfs:comment xml:lang="en">Attribute of some point data set</rdfs:comment>
    </owl:Class>
    


    <!-- http://geographicknowledge.de/vocab/CoreConceptData.rdf#PointData -->

    <owl:Class rdf:about="http://geographicknowledge.de/vocab/CoreConceptData.rdf#PointData">
        <owl:equivalentClass>
            <owl:Class>
                <owl:intersectionOf rdf:parseType="Collection">
                    <rdf:Description rdf:about="http://geographicknowledge.de/vocab/AnalysisData.rdf#SpatialData"/>
                    <owl:Restriction>
                        <owl:onProperty rdf:resource="http://geographicknowledge.de/vocab/GISConcepts.rdf#hasAttribute"/>
                        <owl:someValuesFrom rdf:resource="http://geographicknowledge.de/vocab/CoreConceptData.rdf#Point"/>
                    </owl:Restriction>
                </owl:intersectionOf>
            </owl:Class>
        </owl:equivalentClass>
    </owl:Class>
    


    <!-- http://geographicknowledge.de/vocab/CoreConceptData.rdf#PointDataSet -->

    <owl:Class rdf:about="http://geographicknowledge.de/vocab/CoreConceptData.rdf#PointDataSet">
        <owl:equivalentClass>
            <owl:Class>
                <owl:intersectionOf rdf:parseType="Collection">
                    <rdf:Description rdf:about="http://geographicknowledge.de/vocab/CoreConceptData.rdf#Vector"/>
                    <owl:Restriction>
                        <owl:onProperty rdf:resource="http://geographicknowledge.de/vocab/AnalysisData.rdf#hasElement"/>
                        <owl:allValuesFrom rdf:resource="http://geographicknowledge.de/vocab/CoreConceptData.rdf#PointData"/>
                    </owl:Restriction>
                </owl:intersectionOf>
            </owl:Class>
        </owl:equivalentClass>
        <owl:disjointWith rdf:resource="http://geographicknowledge.de/vocab/CoreConceptData.rdf#RegionDataSet"/>
    </owl:Class>
    


    <!-- http://geographicknowledge.de/vocab/CoreConceptData.rdf#PointMeasures -->

    <owl:Class rdf:about="http://geographicknowledge.de/vocab/CoreConceptData.rdf#PointMeasures">
        <owl:equivalentClass>
            <owl:Class>
                <owl:intersectionOf rdf:parseType="Collection">
                    <rdf:Description rdf:about="http://geographicknowledge.de/vocab/CoreConceptData.rdf#FieldQ"/>
                    <owl:Restriction>
                        <owl:onProperty rdf:resource="http://geographicknowledge.de/vocab/AnalysisData.rdf#ofDataSet"/>
                        <owl:someValuesFrom rdf:resource="http://geographicknowledge.de/vocab/CoreConceptData.rdf#PointDataSet"/>
                    </owl:Restriction>
                </owl:intersectionOf>
            </owl:Class>
        </owl:equivalentClass>
        <rdfs:subClassOf rdf:resource="http://geographicknowledge.de/vocab/CoreConceptData.rdf#FieldVector"/>
        <rdfs:subClassOf rdf:resource="http://geographicknowledge.de/vocab/CoreConceptData.rdf#PointA"/>
        <rdfs:comment xml:lang="en">Point measures are point-like representations of fields. For example, point data sets denoting the locations of measured temperature values.</rdfs:comment>
    </owl:Class>
    


    <!-- http://geographicknowledge.de/vocab/CoreConceptData.rdf#PointMeasuresDS -->

    <owl:Class rdf:about="http://geographicknowledge.de/vocab/CoreConceptData.rdf#PointMeasuresDS">
        <owl:equivalentClass>
            <owl:Class>
                <owl:intersectionOf rdf:parseType="Collection">
                    <rdf:Description rdf:about="http://geographicknowledge.de/vocab/CoreConceptData.rdf#FieldDS"/>
                    <rdf:Description rdf:about="http://geographicknowledge.de/vocab/CoreConceptData.rdf#PointDataSet"/>
                </owl:intersectionOf>
            </owl:Class>
        </owl:equivalentClass>
        <rdfs:subClassOf rdf:resource="http://geographicknowledge.de/vocab/CoreConceptData.rdf#FieldDS"/>
        <rdfs:comment xml:lang="en">A dataset representing a field in terms of point-wise measures. For example, temperature sensor measurements.</rdfs:comment>
    </owl:Class>
    


    <!-- http://geographicknowledge.de/vocab/CoreConceptData.rdf#Raster -->

    <owl:Class rdf:about="http://geographicknowledge.de/vocab/CoreConceptData.rdf#Raster">
        <rdfs:subClassOf rdf:resource="http://geographicknowledge.de/vocab/CoreConceptData.rdf#Tessellation"/>
        <rdfs:comment xml:lang="en">A raster data set is a special kind of tessellation, where regions are regular squares.</rdfs:comment>
    </owl:Class>
    


    <!-- http://geographicknowledge.de/vocab/CoreConceptData.rdf#RasterA -->

    <owl:Class rdf:about="http://geographicknowledge.de/vocab/CoreConceptData.rdf#RasterA">
        <owl:equivalentClass>
            <owl:Class>
                <owl:intersectionOf rdf:parseType="Collection">
                    <rdf:Description rdf:about="http://geographicknowledge.de/vocab/CoreConceptData.rdf#Attribute"/>
                    <owl:Restriction>
                        <owl:onProperty rdf:resource="http://geographicknowledge.de/vocab/AnalysisData.rdf#ofDataSet"/>
                        <owl:someValuesFrom rdf:resource="http://geographicknowledge.de/vocab/CoreConceptData.rdf#Raster"/>
                    </owl:Restriction>
                </owl:intersectionOf>
            </owl:Class>
        </owl:equivalentClass>
        <rdfs:subClassOf rdf:resource="http://geographicknowledge.de/vocab/CoreConceptData.rdf#Attribute"/>
        <rdfs:comment xml:lang="en">Attribute of some Raster</rdfs:comment>
    </owl:Class>
    


    <!-- http://geographicknowledge.de/vocab/CoreConceptData.rdf#RatioA -->

    <owl:Class rdf:about="http://geographicknowledge.de/vocab/CoreConceptData.rdf#RatioA">
        <rdfs:subClassOf rdf:resource="http://geographicknowledge.de/vocab/CoreConceptData.rdf#IntervalA"/>
        <rdfs:comment xml:lang="en">Spatial attribute on ratio scale level</rdfs:comment>
    </owl:Class>
    


    <!-- http://geographicknowledge.de/vocab/CoreConceptData.rdf#Region -->

    <owl:Class rdf:about="http://geographicknowledge.de/vocab/CoreConceptData.rdf#Region">
        <rdfs:subClassOf rdf:resource="http://geographicknowledge.de/vocab/AnalysisData.rdf#Spatial"/>
        <rdfs:comment xml:lang="en">A generalized geometry, including 2D and 3D extended regions. In 2D, this might be a Polygon.</rdfs:comment>
    </owl:Class>
    


    <!-- http://geographicknowledge.de/vocab/CoreConceptData.rdf#RegionA -->

    <owl:Class rdf:about="http://geographicknowledge.de/vocab/CoreConceptData.rdf#RegionA">
        <owl:equivalentClass>
            <owl:Class>
                <owl:intersectionOf rdf:parseType="Collection">
                    <rdf:Description rdf:about="http://geographicknowledge.de/vocab/CoreConceptData.rdf#Attribute"/>
                    <owl:Restriction>
                        <owl:onProperty rdf:resource="http://geographicknowledge.de/vocab/AnalysisData.rdf#ofDataSet"/>
                        <owl:someValuesFrom rdf:resource="http://geographicknowledge.de/vocab/CoreConceptData.rdf#RegionDataSet"/>
                    </owl:Restriction>
                </owl:intersectionOf>
            </owl:Class>
        </owl:equivalentClass>
        <rdfs:subClassOf rdf:resource="http://geographicknowledge.de/vocab/CoreConceptData.rdf#Attribute"/>
        <rdfs:comment xml:lang="en">Atrribute of some region data sets</rdfs:comment>
    </owl:Class>
    


    <!-- http://geographicknowledge.de/vocab/CoreConceptData.rdf#RegionData -->

    <owl:Class rdf:about="http://geographicknowledge.de/vocab/CoreConceptData.rdf#RegionData">
        <owl:equivalentClass>
            <owl:Class>
                <owl:intersectionOf rdf:parseType="Collection">
                    <rdf:Description rdf:about="http://geographicknowledge.de/vocab/AnalysisData.rdf#SpatialData"/>
                    <owl:Restriction>
                        <owl:onProperty rdf:resource="http://geographicknowledge.de/vocab/GISConcepts.rdf#hasAttribute"/>
                        <owl:someValuesFrom rdf:resource="http://geographicknowledge.de/vocab/CoreConceptData.rdf#Region"/>
                    </owl:Restriction>
                </owl:intersectionOf>
            </owl:Class>
        </owl:equivalentClass>
    </owl:Class>
    


    <!-- http://geographicknowledge.de/vocab/CoreConceptData.rdf#RegionDataSet -->

    <owl:Class rdf:about="http://geographicknowledge.de/vocab/CoreConceptData.rdf#RegionDataSet">
        <owl:equivalentClass>
            <owl:Class>
                <owl:intersectionOf rdf:parseType="Collection">
                    <rdf:Description rdf:about="http://geographicknowledge.de/vocab/AnalysisData.rdf#SpatialDataSet"/>
                    <owl:Restriction>
                        <owl:onProperty rdf:resource="http://geographicknowledge.de/vocab/AnalysisData.rdf#hasElement"/>
                        <owl:allValuesFrom rdf:resource="http://geographicknowledge.de/vocab/CoreConceptData.rdf#RegionData"/>
                    </owl:Restriction>
                </owl:intersectionOf>
            </owl:Class>
        </owl:equivalentClass>
    </owl:Class>
    


    <!-- http://geographicknowledge.de/vocab/CoreConceptData.rdf#Tessellation -->

    <owl:Class rdf:about="http://geographicknowledge.de/vocab/CoreConceptData.rdf#Tessellation">
        <rdfs:subClassOf rdf:resource="http://geographicknowledge.de/vocab/CoreConceptData.rdf#RegionDataSet"/>
        <rdfs:comment xml:lang="en">A region data set where spatial regions are tessellated (jointly covering and mutually non-overlapping) within a spatial extent</rdfs:comment>
    </owl:Class>
    


    <!-- http://geographicknowledge.de/vocab/CoreConceptData.rdf#TessellationA -->

    <owl:Class rdf:about="http://geographicknowledge.de/vocab/CoreConceptData.rdf#TessellationA">
        <owl:equivalentClass>
            <owl:Class>
                <owl:intersectionOf rdf:parseType="Collection">
                    <rdf:Description rdf:about="http://geographicknowledge.de/vocab/CoreConceptData.rdf#Attribute"/>
                    <owl:Restriction>
                        <owl:onProperty rdf:resource="http://geographicknowledge.de/vocab/AnalysisData.rdf#ofDataSet"/>
                        <owl:someValuesFrom rdf:resource="http://geographicknowledge.de/vocab/CoreConceptData.rdf#Tessellation"/>
                    </owl:Restriction>
                </owl:intersectionOf>
            </owl:Class>
        </owl:equivalentClass>
        <rdfs:subClassOf rdf:resource="http://geographicknowledge.de/vocab/CoreConceptData.rdf#Attribute"/>
        <rdfs:comment xml:lang="en">An attribute of a tesselation data set</rdfs:comment>
    </owl:Class>
    


    <!-- http://geographicknowledge.de/vocab/CoreConceptData.rdf#Track -->

    <owl:Class rdf:about="http://geographicknowledge.de/vocab/CoreConceptData.rdf#Track">
        <rdfs:subClassOf rdf:resource="http://geographicknowledge.de/vocab/CoreConceptData.rdf#EventVector"/>
        <rdfs:comment xml:lang="en">A type for a spatial track. A spatial track is a vector representation of &quot;fix&quot; events of some moving object. For example, a GPS track of points of a person moving.</rdfs:comment>
    </owl:Class>
    


    <!-- http://geographicknowledge.de/vocab/CoreConceptData.rdf#TrackDS -->

    <owl:Class rdf:about="http://geographicknowledge.de/vocab/CoreConceptData.rdf#TrackDS">
        <rdfs:subClassOf rdf:resource="http://geographicknowledge.de/vocab/CoreConceptData.rdf#EventDS"/>
        <rdfs:subClassOf rdf:resource="http://geographicknowledge.de/vocab/CoreConceptData.rdf#PointDataSet"/>
        <rdfs:comment xml:lang="en">A dataset representing tracks, i.e. point wise events (fixes) of the trajectory of some objects.</rdfs:comment>
    </owl:Class>
    


    <!-- http://geographicknowledge.de/vocab/CoreConceptData.rdf#Vector -->

    <owl:Class rdf:about="http://geographicknowledge.de/vocab/CoreConceptData.rdf#Vector">
        <owl:equivalentClass>
            <owl:Class>
                <owl:intersectionOf rdf:parseType="Collection">
                    <rdf:Description rdf:about="http://geographicknowledge.de/vocab/AnalysisData.rdf#SpatialDataSet"/>
                    <owl:Class>
                        <owl:complementOf rdf:resource="http://geographicknowledge.de/vocab/CoreConceptData.rdf#Raster"/>
                    </owl:Class>
                </owl:intersectionOf>
            </owl:Class>
        </owl:equivalentClass>
        <rdfs:comment xml:lang="en">Vector data sets are spatial data sets that are not raster</rdfs:comment>
    </owl:Class>
    


    <!-- http://geographicknowledge.de/vocab/CoreConceptData.rdf#VectorA -->

    <owl:Class rdf:about="http://geographicknowledge.de/vocab/CoreConceptData.rdf#VectorA">
        <owl:equivalentClass>
            <owl:Class>
                <owl:intersectionOf rdf:parseType="Collection">
                    <rdf:Description rdf:about="http://geographicknowledge.de/vocab/CoreConceptData.rdf#Attribute"/>
                    <owl:Restriction>
                        <owl:onProperty rdf:resource="http://geographicknowledge.de/vocab/AnalysisData.rdf#ofDataSet"/>
                        <owl:someValuesFrom rdf:resource="http://geographicknowledge.de/vocab/CoreConceptData.rdf#Vector"/>
                    </owl:Restriction>
                </owl:intersectionOf>
            </owl:Class>
        </owl:equivalentClass>
        <rdfs:subClassOf rdf:resource="http://geographicknowledge.de/vocab/CoreConceptData.rdf#Attribute"/>
        <rdfs:comment xml:lang="en">Attribute of some vector data set</rdfs:comment>
    </owl:Class>
    


    <!-- http://geographicknowledge.de/vocab/CoreConceptData.rdf#VectorRegionA -->

    <owl:Class rdf:about="http://geographicknowledge.de/vocab/CoreConceptData.rdf#VectorRegionA">
        <owl:equivalentClass>
            <owl:Class>
                <owl:intersectionOf rdf:parseType="Collection">
                    <rdf:Description rdf:about="http://geographicknowledge.de/vocab/CoreConceptData.rdf#RegionA"/>
                    <rdf:Description rdf:about="http://geographicknowledge.de/vocab/CoreConceptData.rdf#VectorA"/>
                </owl:intersectionOf>
            </owl:Class>
        </owl:equivalentClass>
        <rdfs:subClassOf rdf:resource="http://geographicknowledge.de/vocab/CoreConceptData.rdf#Attribute"/>
        <rdfs:comment xml:lang="en">An attribute of a region vector data set</rdfs:comment>
    </owl:Class>
    


    <!-- http://geographicknowledge.de/vocab/CoreConceptData.rdf#VectorTessellation -->

    <owl:Class rdf:about="http://geographicknowledge.de/vocab/CoreConceptData.rdf#VectorTessellation">
        <owl:equivalentClass>
            <owl:Class>
                <owl:intersectionOf rdf:parseType="Collection">
                    <rdf:Description rdf:about="http://geographicknowledge.de/vocab/CoreConceptData.rdf#Tessellation"/>
                    <rdf:Description rdf:about="http://geographicknowledge.de/vocab/CoreConceptData.rdf#Vector"/>
                </owl:intersectionOf>
            </owl:Class>
        </owl:equivalentClass>
        <rdfs:subClassOf rdf:resource="http://geographicknowledge.de/vocab/CoreConceptData.rdf#Tessellation"/>
        <rdfs:comment xml:lang="en">This is a vector data set which is tessellated (and no raster)</rdfs:comment>
    </owl:Class>
    


    <!-- http://geographicknowledge.de/vocab/CoreConceptData.rdf#ZeroExistenceRaster -->

    <owl:Class rdf:about="http://geographicknowledge.de/vocab/CoreConceptData.rdf#ZeroExistenceRaster">
        <rdfs:subClassOf rdf:resource="http://geographicknowledge.de/vocab/CoreConceptData.rdf#ExistenceRaster"/>
        <rdfs:comment xml:lang="en">A raster dataset where 0 is interpreted as boolean &quot;false&quot;</rdfs:comment>
    </owl:Class>
    


    <!-- http://geographicknowledge.de/vocab/ExtensiveMeasures.rdf#ERA -->

    <owl:Class rdf:about="http://geographicknowledge.de/vocab/ExtensiveMeasures.rdf#ERA">
        <rdfs:subClassOf rdf:resource="http://geographicknowledge.de/vocab/CoreConceptData.rdf#IntervalA"/>
        <rdfs:comment xml:lang="en">Extensive region attribute</rdfs:comment>
    </owl:Class>
    


    <!-- http://geographicknowledge.de/vocab/ExtensiveMeasures.rdf#IRA -->

    <owl:Class rdf:about="http://geographicknowledge.de/vocab/ExtensiveMeasures.rdf#IRA">
        <rdfs:subClassOf rdf:resource="http://geographicknowledge.de/vocab/CoreConceptData.rdf#IntervalA"/>
        <rdfs:comment xml:lang="en">Intensive region attribute</rdfs:comment>
    </owl:Class>
    


    <!-- 
    ///////////////////////////////////////////////////////////////////////////////////////
    //
    // Annotations
    //
    ///////////////////////////////////////////////////////////////////////////////////////
     -->

    <rdf:Description rdf:about="http://geographicknowledge.de/vocab/AnalysisData.rdf#measureConnect">
        <rdfs:comment>ofDataSet o hasElement o hasMeasure o valueOf</rdfs:comment>
    </rdf:Description>
    <rdf:Description rdf:about="http://geographicknowledge.de/vocab/AnalysisData.rdf#supportConnect">
        <rdfs:comment>ofDataSet o hasElement o hasSupport o valueOf</rdfs:comment>
    </rdf:Description>
</rdf:RDF>



<!-- Generated by the OWL API (version 4.5.6.2018-09-06T00:27:41Z) https://github.com/owlcs/owlapi -->

